theories/lang/cpp/logic/cclogic.v
@@ -13,7 +13,7 @@ From Coq.Classes Require Import
      RelationClasses Morphisms DecidableClass.
 
 From iris.base_logic.lib Require Import
-     fancy_updates invariants cancelable_invariants own wsat.
+      fancy_updates invariants cancelable_invariants own wsat.
 Import invG.
 From iris.algebra Require Import excl auth.
 
@@ -27,21 +27,16 @@ From bedrock.lang.cpp Require Import
 Section with_Σ.
   Context `{Σ : cpp_logic, !invG Σ}.
 
-  (** Unsound axioms **)
-  (* This should only be possible for wp's for a given mask *)
-  Axiom add_fupd : forall (P : mpred), (|={ ⊤, ⊤ }=> P)%I |-- P.
-
   Section with_Σ'.
     Context `{!inG Σ A}.
 
     Lemma own_alloc_frame (R : A) : forall P Q,
         ✓ R ->
         (forall (γ : gname), P ** own γ R |-- Q) ->
-        P |-- Q.
-    Proof.
+        P |-- |==> Q.
+    Proof using .
       intros.
       iIntros "HP".
-      iApply add_fupd.
       iMod (own_alloc R) as (γ) "H".
       { by apply H. }
       iModIntro.
@@ -51,42 +46,18 @@ Section with_Σ.
 
   End with_Σ'.
 
-  Lemma viewshift_example (P Q : mpred) (N : namespace) :
-    (P -* |={ ⊤ ∖ ↑N, ⊤  }=> Q) ** (|={⊤, ⊤ ∖ ↑N}=> P)%I |--  Q.
-  Proof.
+  Example viewshift_example (P Q : mpred) (N : namespace) :
+    (P -* |={ ⊤ ∖ ↑N, ⊤  }=> Q) ** (|={⊤, ⊤ ∖ ↑N}=> P)%I |-- |={⊤}=> Q.
+  Proof using .
     (* Introduce hypotheses into context by destructing separation conjunct *)
     iIntros "[HPQ HP]".
-    (* Start shifting *)
-    iApply add_fupd.
     (* Construct hypothesis granularity *)
-    iApply (fupd_trans _ (⊤ ∖ ↑N)).
+    iMod "HP".
     (* Resolve second shift *)
     iApply "HPQ".
     (* Resolve first shift *)
     iApply "HP".
   Qed.
-
-  Lemma invariant_example (P : mpred) `{!Persistent P} (N : namespace) : P |-- |> P.
-  Proof.
-    iIntros "HP".
-    (* wp_shift_anywhere *)
-    iApply add_fupd.
-    (* Allocate invariant, using current HP and create new HP (in persistnet context)  *)
-    iMod (inv_alloc N _ (P) with "[HP]") as "#HP".
-    { iNext. eauto. }         (* Solve the goal *)
-    (* Open invariants in namespace N *)
-    iInv N as "#HP'".
-    (* Cancel the reflexive shift *)
-    iModIntro.
-    (* Solve the invariant closing requirement and the goal separately *)
-    iSplitR.
-    - iApply "HP'".
-    - iModIntro. iNext. iApply "HP'".
-  Qed.
-
-  (* notes:
-   * - These can be encoded using ghost state.
-   *)
 
   Context `{!invG Σ}.
 
@@ -98,32 +69,18 @@ Section with_Σ.
 
   Lemma Inv_new : forall n I,
       |>I |-- (|={⊤}=> Inv n I)%I.
-  Proof.
+  Proof using .
     intros. iIntros "HI".
     iApply (inv_alloc with "HI").
   Qed.
 
-  Lemma Inv_dup : forall (n : iname) I, Inv n I -|- Inv n I ** Inv n I.
-  Proof.
-    intros.
-    iSplit.
-    - iIntros "#HI". eauto.
-    - iIntros "[HI _]". eauto.
+  Global Instance: Persistent (Inv n P).
+  Proof using .
+    intros. red. iIntros "#HI". eauto.
   Qed.
 
-  Lemma Inv_drop : forall (n : iname) I, Inv n I |-- empSP.
-  Proof. eauto. Qed.
-
-  (* (* Move this somewhere else? *) *)
-  (* Lemma Inv_new_imp N I : forall (P R Q : mpred), *)
-  (*     (P |-- (|>I) ** R) -> *)
-  (*     Inv N I ** R |-- Q -> *)
-  (*     P |-- Q. *)
-  (* Proof. *)
-  (*   intros. *)
-  (*   rewrite H. rewrite <- H0. rewrite <- (Inv_new N I). *)
-  (*   iIntros "[$ $]". *)
-  (* Qed. *)
+  Global Instance: Affine (Inv n P).
+  Proof using . red. eauto. Qed.
 
   Section with_Σ'.
     Context `{!cinvG Σ}.
@@ -132,46 +89,28 @@ Section with_Σ.
 
     Definition TInv_own γ q : mpred := cinv_own γ q.
 
-    Lemma TInv_new : forall N I,
-        |>I |-- (|={⊤}=> Exists γ, TInv N γ I ** TInv_own γ 1%Qp)%I.
-    Proof.
+    Lemma TInv_new : forall M N I,
+        |>I |-- (|={M}=> Exists γ, TInv N γ I ** TInv_own γ 1%Qp)%I.
+    Proof using .
       intros. iIntros "HI".
       unfold TInv. unfold TInv_own.
         by iApply (cinv_alloc with "[HI]").
     Qed.
 
-    Lemma TInv_dup : forall (N : iname) γ  I,
-        TInv N γ I -|- TInv N γ I ** TInv N γ I.
-    Proof.
-      intros.
-      iSplit.
-      - iIntros "#HI". eauto.
-      - iIntros "[HI _]". eauto.
-    Qed.
-    Lemma TInv_drop : forall (N : iname) γ I, TInv N γ I |-- empSP.
-    Proof. eauto. Qed.
+    Global Instance: Persistent (TInv Ns γ P).
+    Proof using . red. intros; iIntros "#HI". eauto. Qed.
+    Global Instance: Affine (TInv Ns γ P).
+    Proof using . red. eauto. Qed.
 
-    Lemma TInv_delete N γ I :
-      TInv N γ I ** TInv_own γ 1%Qp |-- (|={⊤}=> |>I)%I.
-    Proof.
+    Lemma TInv_delete M N γ I :
+      ↑N ⊆ M ->
+      TInv N γ I ** TInv_own γ 1%Qp |-- (|={M}=> |>I)%I.
+    Proof using .
       intros.
       iIntros "[#Hinv Hq]".
-      iApply add_fupd.
       unfold TInv.
       iApply cinv_cancel; eauto.
     Qed.
-
-    (* Lemma TInv_new_imp N I : forall (P R Q : mpred), *)
-    (*     (P |-- (|>I) ** R) -> *)
-    (*     Exists γ, (TInv N γ I ** TInv_own γ 1%Qp) ** R  |-- Q -> *)
-    (*     P |-- Q. *)
-    (* Proof. *)
-    (*   intros. *)
-    (*   rewrite H. rewrite <- H0. *)
-    (*   rewrite -> (TInv_new N I). *)
-    (*   iIntros "[H $]". *)
-    (*   iDestruct "H" as (γ) "H". eauto. *)
-    (* Qed. *)
 
 
 (*
@@ -203,7 +142,7 @@ Section with_Σ.
       cinv N γ P |--
            (cinv_own γ p ={E,E∖↑N}=∗
                                   ((|>P) ** cinv_own γ p ** (Forall (E' : coPset), ((|>P ∨ cinv_own γ 1) ={E',↑N ∪ E'}=∗ True))))%I.
-    Proof. iIntros (?) "#Hinv Hown". iApply cinv_acc_strong =>//. Qed.
+    Proof using . iIntros (?) "#Hinv Hown". iApply cinv_acc_strong =>//. Qed.
 
   End with_Σ'.
 End with_Σ.
