theories/lang/cpp/logic/destructors.v
@@ -11,14 +11,13 @@ From bedrock.lang.cpp.logic Require Import
 
 Section with_resolve.
   Context `{Σ : cpp_logic thread_info} {σ: genv}.
-  Variable ti : thread_info.
-  Variable ρ : region.
+  Variables (M : coPset) (ti : thread_info) (ρ : region).
 
   Axiom wpd_deinit : forall (cls : globname) (this : val) path dn (Q : epred),
     Exists dp, Exists fp,
       (@_global σ dn &~ dp **
        _offsetL (offset_for σ cls path) (_eqv this) &~ fp ** ltrue) //\\
       (|> fspec ti (Vptr dp) (this :: nil) (fun _ => Q))
-    |-- wpd (resolve:=σ) ti ρ cls this (path, dn) Q.
+    |-- wpd (resolve:=σ) M ti ρ cls this (path, dn) Q.
 
 End with_resolve.
