theories/lang/cpp/logic/initializers.v
@@ -17,17 +17,17 @@ Module Type Init.
 
   Section with_resolve.
     Context `{Σ : cpp_logic thread_info} {σ:genv}.
-    Variables (ti : thread_info) (ρ : region).
+    Variables (M : coPset) (ti : thread_info) (ρ : region).
 
-    Local Notation wp := (wp (resolve:=σ) ti ρ).
-    Local Notation wpi := (wpi (resolve:=σ) ti ρ).
-    Local Notation wpe := (wpe (resolve:=σ) ti ρ).
-    Local Notation wp_lval := (wp_lval (resolve:=σ) ti ρ).
-    Local Notation wp_rval := (wp_rval (resolve:=σ) ti ρ).
-    Local Notation wp_prval := (wp_prval (resolve:=σ) ti ρ).
-    Local Notation wp_xval := (wp_xval (resolve:=σ) ti ρ).
-    Local Notation wp_init := (wp_init (resolve:=σ) ti ρ).
-    Local Notation wp_args := (wp_args (σ:=σ) ti ρ).
+    Local Notation wp := (wp (resolve:=σ) M ti ρ).
+    Local Notation wpi := (wpi (resolve:=σ) M ti ρ).
+    Local Notation wpe := (wpe (resolve:=σ) M ti ρ).
+    Local Notation wp_lval := (wp_lval (resolve:=σ) M ti ρ).
+    Local Notation wp_rval := (wp_rval (resolve:=σ) M ti ρ).
+    Local Notation wp_prval := (wp_prval (resolve:=σ) M ti ρ).
+    Local Notation wp_xval := (wp_xval (resolve:=σ) M ti ρ).
+    Local Notation wp_init := (wp_init (resolve:=σ) M ti ρ).
+    Local Notation wp_args := (wp_args (σ:=σ) M ti ρ).
     Local Notation fspec := (fspec ti).
 
     Local Notation _global := (_global (resolve:=σ)) (only parsing).
