theories/lang/cpp/logic/linking.v
@@ -11,81 +11,26 @@ From bedrock.lang.cpp Require Import
      ast logic.pred logic.compilation_unit.
 
 Section with_PROP.
-Context {PROP : sbi}.
+  Context {PROP : sbi}.
 
-Lemma illater_wandSP : forall (P Q : PROP), |> (P -* Q) |-- (|> P) -* (|> Q).
-Proof.
-  iIntros (P Q). iIntros "HPQ HP". iNext. by iApply "HPQ".
-Qed.
-Lemma illater_sepSP : forall (P Q : PROP), |> (P ** Q) -|- (|> P) ** (|> Q).
-Proof.
-  iIntros (P Q). iSplit.
-  - iIntros "HPQ". by iApply bi.later_sep_1.
-  - iIntros "HPQ". iNext. eauto.
-Qed.
-(* Lemma later_empSP : |> (empSP : PROP) -|- empSP. *)
-(* Proof. apply bi.later_emp. SearchAbout sbi_later. Qed. *)
+  Lemma illater_wandSP : forall (P Q : PROP), |> (P -* Q) |-- (|> P) -* (|> Q).
+  Proof.
+    iIntros (P Q). iIntros "HPQ HP". iNext. by iApply "HPQ".
+  Qed.
+  Lemma illater_sepSP : forall (P Q : PROP), |> (P ** Q) -|- (|> P) ** (|> Q).
+  Proof.
+    iIntros (P Q). iSplit.
+    - iIntros "HPQ". by iApply bi.later_sep_1.
+    - iIntros "HPQ". iNext. eauto.
+  Qed.
 
-(* note that the meaning of a module must be persistent,
- * if you have non-persistent terms (e.g. ptsto), then you either need
- * to put them inside invariants, or prove that they do not depend on
- * the imports (this would only be a problem if they are initialized via
- * a function call, but I don't think that you can actually do that).
- *)
-Definition module (imports exports : PROP) : PROP :=
-  (|> imports) -* exports.
+  (* note that the meaning of a module must be persistent,
+   * if you have non-persistent terms (e.g. ptsto), then you either need
+   * to put them inside invariants, or prove that they do not depend on
+   * the imports (this would only be a problem if they are initialized via
+   * a function call, but I don't think that you can actually do that).
+   *)
+  Definition module (imports exports : PROP) : PROP :=
+    (|> imports) -* exports.
 
-(* Theorem use_module_prim *)
-(* : forall (all sub rem : compilation_unit) spec, *)
-(*     match link sub rem with *)
-(*     | None => False *)
-(*     | Some all' => compilation_unit_eq all all' = true *)
-(*     end -> *)
-(*     denoteModule (Σ := Σ) sub |-- spec -> *)
-(*     denoteModule all |-- denoteModule rem ** spec. *)
-(* Proof. Admitted. *)
-
-
-(*
-Theorem module_self_link (E : PROP) :
-  module E E |-- E.
-Proof.
-  eapply lob_ind.
-  unfold module.
-  eapply landAdj.
-  reflexivity.
-Qed.
-
-Theorem module_link (I1 I2 E1 E2 : PROP) :
-  module (E2 ** I1) E1 ** module (E1 ** I2) E2
-  |-- module (I1 ** I2) (E1 ** E2).
-Proof. Abort.
-
-Lemma lob_link : forall A B : PROP,
-    ((|> A) -->> B) //\\ ((|> B) -->> A) |-- A //\\ B.
-Proof.
-  intros. (*
-  eapply sepSPAdj'.
-  rewrite <- empSPL.
-  eapply sepSPAdj.
-  rewrite <- (landtrueR empSP).
-  apply landL2.
-  rewrite <- wand_curry.
-  eapply wandSPAdj.
-  eapply lob_ind.
-  rewrite illater_sepSP.
-  eapply spec_lob.
-  eapply wandSPAdj.
-  eapply wandSPE.
-  reflexivity.
-  eapply scME.
-  instantiate (1:=|> ((|> B) -* A) ** ((|> A))).
-*)
-
-Abort.
-*)
-    (* |>A ==> B
-     * |>B ==> A
-     * A //\\ B
-     *)
 End with_PROP.
