theories/lang/cpp/logic_notations.v
@@ -8,43 +8,43 @@
 Require Import bedrock.lang.cpp.logic.
 
 Module Compact.
-Notation "'::wpL' { e }" := (@wp_lval _ _ _ _ _ e _)
+Notation "'::wpL' { e }" := (@wp_lval _ _ _ _ _ _ e _)
          (at level 0, only printing).
-Notation "'::wpX' { e }" := (@wp_xval _ _ _ _ _ e _)
+Notation "'::wpX' { e }" := (@wp_xval _ _ _ _ _ _ e _)
          (at level 0, only printing).
-Notation "'::wpPR' { e }" := (@wp_prval _ _ _ _ _ e _)
+Notation "'::wpPR' { e }" := (@wp_prval _ _ _ _ _ _ e _)
          (at level 0, only printing).
-Notation "'::wpPRᵢ' { e }" := (@wp_init _ _ _ _ _ _ _ e _)
+Notation "'::wpPRᵢ' { e }" := (@wp_init _ _ _ _ _ _ _ _ e _)
          (at level 0, only printing).
-Notation "'::wpGL' { e }" := (@wp_glval _ _ _ _ _ e _)
+Notation "'::wpGL' { e }" := (@wp_glval _ _ _ _ _ _ e _)
          (at level 0, only printing).
-Notation "'::wpR' { e }" := (@wp_rval _ _ _ _ _ e _)
+Notation "'::wpR' { e }" := (@wp_rval _ _ _ _ _ _ e _)
          (at level 0, only printing).
-Notation "'::wpS' { e }" := (@wp _ _ _ _ _ e _)
+Notation "'::wpS' { e }" := (@wp _ _ _ _ _ _ e _)
          (at level 0, only printing).
-Notation "'::wpE' { e }" := (@wpe _ _ _ _ _ _ e _)
+Notation "'::wpE' { e }" := (@wpe _ _ _ _ _ _ _ e _)
          (at level 0, only printing).
-Notation "'::wpD' { t n = e }" := (@wp_decl _ _ _ _ _ n t e _ _ _)
+Notation "'::wpD' { t n = e }" := (@wp_decl _ _ _ _ _ _ n t e _ _ _)
          (at level 0, only printing).
 End Compact.
 
 Module Verbose.
-Notation "'::wpL' { e } Q" := (@wp_lval _ _ _ _ _ e Q)
+Notation "'::wpL' { e } Q" := (@wp_lval _ _ _ _ _ _ e Q)
          (at level 0, Q at level 200, only printing).
-Notation "'::wpX' { e } Q" := (@wp_xval _ _ _ _ _ e Q)
+Notation "'::wpX' { e } Q" := (@wp_xval _ _ _ _ _ _ e Q)
          (at level 0, Q at level 200, only printing).
-Notation "'::wpPR' { e } Q" := (@wp_prval _ _ _ _ _ e Q)
+Notation "'::wpPR' { e } Q" := (@wp_prval _ _ _ _ _ _ e Q)
          (at level 0, Q at level 200, only printing).
-Notation "'::wpPRᵢ' { e } Q" := (@wp_init _ _ _ _ _ _ _ e Q)
+Notation "'::wpPRᵢ' { e } Q" := (@wp_init _ _ _ _ _ _ _ _ e Q)
          (at level 0, Q at level 200, only printing).
-Notation "'::wpGL' { e } Q" := (@wp_glval _ _ _ _ _ e Q)
+Notation "'::wpGL' { e } Q" := (@wp_glval _ _ _ _ _ _ e Q)
          (at level 0, Q at level 200, only printing).
-Notation "'::wpR' { e } Q" := (@wp_rval _ _ _ _ _ e Q)
+Notation "'::wpR' { e } Q" := (@wp_rval _ _ _ _ _ _ e Q)
          (at level 0, Q at level 200, only printing).
-Notation "'::wpS' { e } Q" := (@wp _ _ _ _ _ e Q)
+Notation "'::wpS' { e } Q" := (@wp _ _ _ _ _ _ e Q)
          (at level 0, Q at level 200, only printing).
-Notation "'::wpE' { e } Q" := (@wpe _ _ _ _ _ _ e Q)
+Notation "'::wpE' { e } Q" := (@wpe _ _ _ _ _ _ _ e Q)
          (at level 0, Q at level 200, only printing).
-Notation "'::wpD' { t n = e } Q" := (@wp_decl _ _ _ _ _ n t e _ _ Q)
+Notation "'::wpD' { t n = e } Q" := (@wp_decl _ _ _ _ _ _ n t e _ _ Q)
          (at level 0, Q at level 200, only printing).
 End Verbose.
